Prove recursive vacuity soundness

VisualProof/Rule/Vacuity.lean
@@ -26,4 +26,16 @@ inductive Local : LocalRule
 
 end Vacuity
 
+def Vacuity : Rule :=
+  Contextual (symmetric Vacuity.Local)
+
+theorem Vacuity.iso
+    {arity : Nat}
+    {source source' target target' : OpenDiagram arity}
+    (sourceIso : OpenDiagramIso source source')
+    (step : Vacuity source target)
+    (targetIso : OpenDiagramIso target target') :
+    Vacuity source' target' :=
+  Contextual.iso sourceIso step targetIso
+
 end VisualProof.Rule
